Moved to separate syntex system. Noticed i forgot about DoBind

language_formalisation/operational_semantics/operational_semantics.v
@@ -4,44 +4,44 @@ Add LoadPath "C:\Users\Ziga\Documents\Ziga_podatki\PHD\language_formalisation\su
 (* Add Rec LoadPath "E:\Ziga_Podatki\faks\PHD\language_formalisation\substitution". *)
 Require Export syntax substitution.
 
-Inductive small_step : comp -> comp -> Type :=
-| Step_pmatch v1 v2 x y c: 
-    small_step 
+Inductive step : comp -> comp -> Prop :=
+| Step_ΠMatch v1 v2 x y c: 
+    step 
       (ΠMatch (Pair v1 v2) (x, y) c)
       (c_sub2_out c v1 v2)
-| Step_smatch_l v xl cl xr cr:
-    small_step 
+| Step_ΣMatch_Inl v xl cl xr cr:
+    step 
       (ΣMatch (Inl v) xl cl xr cr)
       (c_sub_out cl v)
-| Step_smatch_r v xl cl xr cr:
-    small_step 
+| Step_ΣMatch_Inr v xl cl xr cr:
+    step 
       (ΣMatch (Inr v) xl cl xr cr)
       (c_sub_out cr v)
-| Step_apply x c v:
-    small_step (App (Fun x c) v) (c_sub_out c v)
-| Step_dobind_step x c1 c1' c2:
-    small_step c1 c1' ->
-    small_step (DoBind x c1 c2) (DoBind x c1' c2)
-| Step_letrec f x f_ty c1 c2:
-    small_step
-      (LetRec f x f_ty c1 c2)
-      (c_sub_out c2 (Fun x (LetRec f x f_ty (Sub.c_shift c1 1 2) c1)))
-| Step_dobind_ret x v c:
-    small_step (DoBind x (Ret v) c) (c_sub_out c v)
-| Step_dobind_op x op_id v_arg y c1 c2:
-    small_step
+| Step_App x c v:
+    step (App (Fun x c) v) (c_sub_out c v)
+| Step_LetRec f x c1 c2:
+    step
+      (LetRec f x c1 c2)
+      (c_sub_out c2 (Fun x (LetRec f x (Sub.c_shift c1 1 2) c1)))
+| Step_DoBind_step x c1 c1' c2:
+    step c1 c1' ->
+    step (DoBind x c1 c2) (DoBind x c1' c2)
+| Step_DoBind_Ret x v c:
+    step (DoBind x (Ret v) c) (c_sub_out c v)
+| Step_DoBind_Op x op_id v_arg y c1 c2:
+    step
       (DoBind x (Op op_id v_arg y c1) c2)
       (Op op_id v_arg y (DoBind x c1 c2))
-| Step_handle_step v c c' :
-    small_step c c' ->
-    small_step (Handle v c) (Handle v c')
-| Step_handle_ret x c_r h v :
-    small_step
+| Step_Handle_Step v c c' :
+    step c c' ->
+    step (Handle v c) (Handle v c')
+| Step_Handle_Ret x c_r h v :
+    step
       (Handle (Handler x c_r h) (Ret v))
       (c_sub_out c_r v)
-| Step_handle_op x c_r h op_id v_arg y c_k x_op k_op c_op :
+| Step_Handle_Op x c_r h op_id v_arg y c_k x_op k_op c_op :
     find_op_case h op_id = Some (x_op, k_op, c_op) ->
-    small_step
+    step
       (Handle (Handler x c_r h) (Op op_id v_arg y c_k))
       (c_sub2_out c_op
         (Fun y (Handle (Sub.v_shift (Handler x c_r h) 1 0) c_k))
