language_formalisation/type_system/bidirectional.v
@@ -2,77 +2,77 @@ Add LoadPath "C:\Users\Ziga\Documents\Ziga_podatki\PHD\language_formalisation\sy
 (* Add LoadPath "E:\Ziga_Podatki\faks\PHD\language_formalisation\syntax". *)
 Require Import syntax.
 
-Inductive vsynth : ctx -> val -> vtype -> Prop :=
-| SynthUnit Γ : vsynth Γ Unit TyUnit 
-| SynthInt Γ n : vsynth Γ (Int n) TyInt
-| SynthVar Γ id A :
-    get_vtype Γ id = Some A ->
-    vsynth Γ (Var id) A
+Inductive vsynth : ctx -> ann_val -> vtype -> Prop :=
+| SynthUnit Γ : vsynth Γ Ann_Unit TyUnit 
+| SynthInt Γ n : vsynth Γ (Ann_Int n) TyInt
+| SynthVar Γ name num A :
+    get_vtype Γ num = Some A ->
+    vsynth Γ (Ann_Var (name, num)) A
 | SynthPair Γ v1 v2 A B :
     vsynth Γ v1 A ->
     vsynth Γ v2 B ->
-    vsynth Γ (Pair v1 v2) (TyΠ A B)
+    vsynth Γ (Ann_Pair v1 v2) (TyΠ A B)
 | SynthVAnnot Γ v A :
     vcheck Γ v A ->
-    vsynth Γ (VAnnot v A) A
-with csynth : ctx -> comp -> ctype -> Prop :=
+    vsynth Γ (Ann_Val v A) A
+with csynth : ctx -> ann_comp -> ctype -> Prop :=
 | SynthRet Γ v A : 
     vsynth Γ v A ->
-    csynth Γ (Ret v) (CTy A SigØ EqsØ)
+    csynth Γ (Ann_Ret v) (CTy A SigØ EqsØ)
 | SynthΠMatch Γ v A B x y c C :
     vsynth Γ v (TyΠ A B) ->
     csynth (CtxU (CtxU Γ A) B) c C ->
-    csynth Γ (ΠMatch v (x, y) c) C
+    csynth Γ (Ann_ΠMatch v (x, y) c) C
 | SynthApp Γ v1 v2 A C :
     vsynth Γ v1 (TyFun A C) ->
     vcheck Γ v2 A ->
-    csynth Γ (App v1 v2) C
+    csynth Γ (Ann_App v1 v2) C
 | SynthHandle Γ v c C D :
     vsynth Γ v (TyHandler C D) ->
     ccheck Γ c C ->
-    csynth Γ (Handle v c) D
+    csynth Γ (Ann_Handle v c) D
 | SynthCAnnot Γ c C :
     ccheck Γ c C ->
-    csynth Γ (CAnnot c C) C
+    csynth Γ (Ann_Comp c C) C
 | SynthLetRec Γ f x A C c1 c2 D:
     ccheck (CtxU (CtxU Γ A) (TyFun A C)) c1 C ->
     csynth (CtxU Γ (TyFun A C)) c2 D ->
-    csynth Γ (LetRec f x (TyFun A C) c1 c2) D
+    csynth Γ (Ann_LetRec f x (TyFun A C) c1 c2) D
 (* with hsynth : ctx -> hcases -> sig -> ctype -> Type := *)
-with vcheck : ctx -> val -> vtype -> Prop :=
+with vcheck : ctx -> ann_val -> vtype -> Prop :=
 | CheckVBySynth Γ v A : vsynth Γ v A -> vcheck Γ v A
 | CheckInl Γ v A B :
     vcheck Γ v A ->
-    vcheck Γ (Inl v) (TyΣ A B)
+    vcheck Γ (Ann_Inl v) (TyΣ A B)
 | CheckInr Γ v A B :
     vcheck Γ v B ->
-    vcheck Γ (Inr v) (TyΣ A B)
+    vcheck Γ (Ann_Inr v) (TyΣ A B)
 | CheckFun Γ x c A C :
     ccheck (CtxU Γ A) c C ->
-    vcheck Γ (Fun x c) (TyFun A C)
+    vcheck Γ (Ann_Fun x c) (TyFun A C)
 | CheckHandler Γ x c_ret h A sig eqs D :
     ccheck (CtxU Γ A) c_ret D ->
     hcheck Γ h sig D ->
-    vcheck Γ (Handler x c_ret h) (TyHandler (CTy A sig eqs) D)
-with ccheck : ctx -> comp -> ctype -> Prop :=
+    vcheck Γ (Ann_Handler x c_ret h) (TyHandler (CTy A sig eqs) D)
+with ccheck : ctx -> ann_comp -> ctype -> Prop :=
 | CheckCBySynth Γ c C C' : csynth Γ c C' -> C = C' -> ccheck Γ c C
 | CheckΣMatch Γ v A B xl cl xr cr C :
     vsynth Γ v (TyΣ A B) ->
     ccheck (CtxU Γ A) cl C ->
     ccheck (CtxU Γ B) cr C ->
-    ccheck Γ (ΣMatch v xl cl xr cr) C
+    ccheck Γ (Ann_ΣMatch v xl cl xr cr) C
 | CheckOp Γ op_id v y c A_op B_op A Σ eqs :
     get_op_type Σ op_id = Some (A_op, B_op) ->
     vcheck Γ v A_op ->
     ccheck (CtxU Γ B_op) c (CTy A Σ eqs) ->
-    ccheck Γ (Op op_id v y c) (CTy A Σ eqs)
-with hcheck : ctx -> hcases -> sig -> ctype -> Prop :=
-| CheckCasesØ Γ D : hcheck Γ CasesØ SigØ D
+    ccheck Γ (Ann_Op op_id v y c) (CTy A Σ eqs)
+with hcheck : ctx -> ann_hcases -> sig -> ctype -> Prop :=
+| CheckCasesØ Γ D : hcheck Γ Ann_CasesØ SigØ D
 | CheckCasesU Γ h op_id x k c_op A_op B_op Σ D :
-    find_op_case h op_id = None ->
+    find_op_ann_case h op_id = None ->
     hcheck Γ h Σ D ->
     ccheck (CtxU (CtxU Γ (TyFun B_op D)) A_op) c_op D ->
     hcheck 
-      Γ (CasesU h op_id x k c_op)
+      Γ (Ann_CasesU h op_id x k c_op)
       (SigU Σ op_id A_op B_op) D
 .
