language_formalisation/type_system/declarational.v
@@ -2,21 +2,18 @@ Add LoadPath "C:\Users\Ziga\Documents\Ziga_podatki\PHD\language_formalisation\sy
 Add LoadPath "C:\Users\Ziga\Documents\Ziga_podatki\PHD\language_formalisation\type_system".
 (* Add LoadPath "E:\Ziga_Podatki\faks\PHD\language_formalisation\syntax". *)
 (* Add LoadPath "E:\Ziga_Podatki\faks\PHD\language_formalisation\type_system". *)
-Require Import syntax bidirectional.
+Require Import syntax syntax_lemmas bidirectional.
 
 Inductive has_vtype : ctx -> val -> vtype -> Prop :=
 | TypeUnit Γ : has_vtype Γ Unit TyUnit 
 | TypeInt Γ n : has_vtype Γ (Int n) TyInt
-| TypeVar Γ id A :
-    get_vtype Γ id = Some A ->
-    has_vtype Γ (Var id) A
+| TypeVar Γ name num A :
+    get_vtype Γ num = Some A ->
+    has_vtype Γ (Var (name, num)) A
 | TypePair Γ v1 v2 A B :
     has_vtype Γ v1 A ->
     has_vtype Γ v2 B ->
     has_vtype Γ (Pair v1 v2) (TyΠ A B)
-| TypeVAnnot Γ v A :
-    has_vtype Γ v A ->
-    has_vtype Γ (VAnnot v A) A
 | TypeInl Γ v A B :
     has_vtype Γ v A ->
     has_vtype Γ (Inl v) (TyΣ A B)
@@ -46,13 +43,10 @@ with has_ctype : ctx -> comp -> ctype -> Prop :=
     has_vtype Γ v (TyHandler C D) ->
     has_ctype Γ c C ->
     has_ctype Γ (Handle v c) D
-| TypeCAnnot Γ c C :
-    has_ctype Γ c C ->
-    has_ctype Γ (CAnnot c C) C
 | TypeLetRec Γ f x A C c1 c2 D:
     has_ctype (CtxU (CtxU Γ A) (TyFun A C)) c1 C ->
     has_ctype (CtxU Γ (TyFun A C)) c2 D ->
-    has_ctype Γ (LetRec f x (TyFun A C) c1 c2) D
+    has_ctype Γ (LetRec f x c1 c2) D
 | TypeΣMatch Γ v A B xl cl xr cr C :
     has_vtype Γ v (TyΣ A B) ->
     has_ctype (CtxU Γ A) cl C ->
@@ -73,285 +67,3 @@ with has_htype : ctx -> hcases -> sig -> ctype -> Prop :=
       Γ (CasesU h op_id x k c_op)
       (SigU Σ op_id A_op B_op) D
 .
-
-Ltac inv H := inversion H; clear H; subst.
-
-
-Fixpoint vcheck_has_vtype Γ v A {struct v}:
-  vcheck Γ v A -> has_vtype Γ v A
-with vsynth_has_vtype Γ v A {struct v}:
-  vsynth Γ v A -> has_vtype Γ v A
-with ccheck_has_ctype Γ c C {struct c}:
-  ccheck Γ c C -> has_ctype Γ c C
-with csynth_has_ctype Γ c C {struct c}:
-  csynth Γ c C -> has_ctype Γ c C
-with hcheck_has_htype Γ h Σ D {struct h}:
-  hcheck Γ h Σ D -> has_htype Γ h Σ D.
-Proof.
-{
-clear vcheck_has_vtype.
-revert Γ A. induction v; intros Γ A orig; inv orig; try inv H.
-+ apply TypeVar. assumption.
-+ apply TypeUnit.
-+ apply TypeInt.
-+ apply TypeInl. apply IHv. assumption.
-+ apply TypeInr. apply IHv. assumption.
-+ apply TypePair; auto.
-+ apply TypeFun. auto.
-+ apply TypeHandler; auto.
-+ apply TypeVAnnot; auto.
-}{
-clear vsynth_has_vtype.
-revert Γ A. induction v; intros Γ A orig; inv orig.
-+ apply TypeVar. assumption.
-+ apply TypeUnit.
-+ apply TypeInt.
-+ apply TypePair; auto.
-+ apply TypeVAnnot. auto.
-}{
-clear ccheck_has_ctype.
-revert Γ C. induction c; intros Γ C orig; inv orig; try inv H.
-+ apply TypeRet. auto.
-+ eapply TypeΠMatch. apply vsynth_has_vtype; exact H5.
-  apply csynth_has_ctype. assumption.
-+ eapply TypeΣMatch. apply vsynth_has_vtype; exact H6. auto. auto.
-+ eapply TypeApp. apply vsynth_has_vtype. exact H3. auto.
-+ eapply TypeOp; try exact H5 || auto.
-+ apply TypeLetRec; auto.
-+ eapply TypeHandle. apply vsynth_has_vtype. exact H3. auto.
-+ apply TypeCAnnot. auto. 
-}{
-clear csynth_has_ctype.
-revert Γ C. induction c; intros Γ C orig; inv orig.
-+ apply TypeRet. auto.
-+ eapply TypeΠMatch. apply vsynth_has_vtype; exact H4. auto.
-+ eapply TypeApp. apply vsynth_has_vtype; exact H2. auto.
-+ apply TypeLetRec. auto. apply IHc2. assumption.
-+ eapply TypeHandle. apply vsynth_has_vtype; exact H2. auto.
-+ eapply TypeCAnnot. auto.
-}{
-clear hcheck_has_htype.
-revert Γ Σ D. induction h; intros Γ Σ D orig; inv orig.
-+ apply TypeCasesØ.
-+ apply TypeCasesU; auto.
-}
-Qed.
-
-
-Fixpoint v_remove_annot v :=
-match v with
-| Var id => Var id
-| Unit => Unit
-| Int n => Int n
-| Inl v' => Inl (v_remove_annot v')
-| Inr v' => Inr (v_remove_annot v')
-| Pair v1 v2 => Pair (v_remove_annot v1) (v_remove_annot v2)
-| Fun x c => Fun x (c_remove_annot c)
-| Handler x c_ret h => Handler x (c_remove_annot c_ret) (h_remove_annot h)
-| VAnnot v' A => v_remove_annot v'
-end
-with c_remove_annot c :=
-match c with
-| Ret v => Ret (v_remove_annot v)
-| ΠMatch v (x, y) c => ΠMatch (v_remove_annot v) (x,y) (c_remove_annot c)
-| ΣMatch v xl cl xr cr => 
-    ΣMatch (v_remove_annot v) xl (c_remove_annot cl) xr (c_remove_annot cr)
-| App v1 v2 => App (v_remove_annot v1) (v_remove_annot v2)
-| Op op v_arg y c => Op op (v_remove_annot v_arg) y (c_remove_annot c)
-| LetRec f x f_ty c1 c2 =>
-    LetRec f x f_ty (c_remove_annot c1) (c_remove_annot c2)
-| DoBind x c1 c2 => DoBind x (c_remove_annot c1) (c_remove_annot c2)
-| Handle v c' => Handle (v_remove_annot v) (c_remove_annot c')
-| CAnnot c' C => (c_remove_annot c')
-end
-with h_remove_annot h :=
-match h with
-| CasesØ => CasesØ
-| CasesU h op x k c =>
-    CasesU (h_remove_annot h) op x k (c_remove_annot c)
-end.
-
-Lemma v_type_remove_annot Γ v A:
-  has_vtype Γ v A -> has_vtype Γ (v_remove_annot v) A
-with c_type_remove_annot Γ c C:
-  has_ctype Γ c C -> has_ctype Γ (c_remove_annot c) C
-with h_type_remove_annot Γ h Σ D:
-  has_htype Γ h Σ D -> has_htype Γ (h_remove_annot h) Σ D.
-Proof.
-{
-revert Γ A. induction v; intros Γ A orig; inv orig; simpl; auto.
-+ apply TypeVar. assumption.
-+ apply TypeUnit.
-+ apply TypeInt.
-+ apply TypeInl. apply IHv. assumption.
-+ apply TypeInr. apply IHv. assumption.
-+ apply TypePair; auto.
-+ apply TypeFun. auto.
-+ apply TypeHandler; auto.
-}{
-revert Γ C. induction c; intros Γ C orig; inv orig; simpl; auto.
-+ apply TypeRet. auto.
-+ eapply TypeΠMatch. apply v_type_remove_annot. exact H4.
-  apply c_type_remove_annot. assumption.
-+ eapply TypeΣMatch. apply v_type_remove_annot. exact H6. auto. auto.
-+ eapply TypeApp. apply v_type_remove_annot. exact H2. auto.
-+ eapply TypeOp; try exact H5 || auto.
-+ apply TypeLetRec; auto.
-+ eapply TypeHandle. apply v_type_remove_annot. exact H2. auto.
-}{
-revert Γ Σ D. induction h; intros Γ Σ D orig; inv orig; simpl; auto.
-+ apply TypeCasesØ.
-+ apply TypeCasesU; auto.
-  assert (forall h o,
-    find_op_case h o = None -> find_op_case (h_remove_annot h) o = None).
-  { intros h' op orig. induction h'.
-    * simpl. auto.
-    * simpl. simpl in *. destruct (op == o0).
-      ++ discriminate.
-      ++ auto.
-  }
-  apply H. auto.
-}
-Qed.
-
-
-Fixpoint has_vtype_vsynths_with_annot Γ v A {struct v}:
-  has_vtype Γ v A -> 
-    exists v', vsynth Γ v' A /\ v_remove_annot v = v_remove_annot v'
-with has_ctype_csynths_with_annot Γ c C {struct c}:
-  has_ctype Γ c C ->
-    exists c', csynth Γ c' C /\ c_remove_annot c = c_remove_annot c'
-with has_htype_hchecks_with_annot Γ h Σ D {struct h}:
-  has_htype Γ h Σ D ->
-    exists h', hcheck Γ h' Σ D /\ h_remove_annot h = h_remove_annot h'.
-Proof.
-all:
-rename has_vtype_vsynths_with_annot into vLemma;
-rename has_ctype_csynths_with_annot into cLemma;
-rename has_htype_hchecks_with_annot into hLemma.
-{
-clear vLemma.
-revert Γ A. induction v; intros Γ A orig.
-- exists (Var v). constructor.
-  + apply SynthVar. inv orig. assumption.
-  + reflexivity.
-- exists Unit. constructor.
-  + inv orig. apply SynthUnit.
-  + reflexivity.
-- exists (Int t). constructor.
-  + inv orig. apply SynthInt.
-  + reflexivity.
-- (* Annotate sumtypes *)
-  inv orig. apply IHv in H1. destruct H1 as [v' [vty' same]].
-  exists (VAnnot (Inl v') (TyΣ A0 B)). constructor.
-  + apply SynthVAnnot. apply CheckInl. apply CheckVBySynth. assumption.
-  + simpl. f_equal. assumption.
-- (* Annotate sumtypes *)
-  inv orig. apply IHv in H1. destruct H1 as [v' [vty' same]].
-  exists (VAnnot (Inr v') (TyΣ A0 B)). constructor.
-  + apply SynthVAnnot. apply CheckInr. apply CheckVBySynth. assumption.
-  + simpl. f_equal. assumption.
-- inv orig.
-  apply IHv1 in H2. destruct H2 as [v1' [v1ty' same1]].
-  apply IHv2 in H4. destruct H4 as [v2' [v2ty' same2]].
-  exists (Pair v1' v2'). constructor.
-  + apply SynthPair; assumption.
-  + simpl. f_equal; assumption.
-- inv orig. (* Annotate functions. *)
-  apply cLemma in H3. destruct H3 as [c' [cty' same]].
-  exists (VAnnot (Fun v c') (TyFun A0 C)). constructor.
-  + apply SynthVAnnot. apply CheckFun. eapply CheckCBySynth. exact cty'. auto.
-  + simpl. f_equal. assumption.
-- inv orig. (* Annotate functions. *)
-  apply cLemma in H4. destruct H4 as [c_r' [cty' samec]].
-  apply hLemma in H5. destruct H5 as [h' [hty' sameh]].
-  exists (VAnnot (Handler v c_r' h') (TyHandler (CTy A0 sig eqs) D)).
-  constructor.
-  + apply SynthVAnnot. apply CheckHandler;
-    try eapply CheckCBySynth; auto. auto.
-  + simpl. f_equal; assumption.
-- inv orig. apply IHv in H3. destruct H3 as [v' [vty' same1]].
-  exists (VAnnot v' A). constructor.
-  + apply SynthVAnnot. apply CheckVBySynth. assumption.
-  + simpl. assumption.
-}{
-clear cLemma.
-revert Γ C. induction c; intros Γ C orig.
-- inv orig.
-  apply vLemma in H1. destruct H1 as [v' [vty' same]].
-  exists (Ret v'). constructor.
-  + apply SynthRet. assumption.
-  + simpl. f_equal. assumption.
-- inv orig.
-  apply vLemma in H4. destruct H4 as [v' [vty' same]].
-  apply IHc in H5. destruct H5 as [c' [cty' csame]].
-  exists (ΠMatch v' (x,y) c'). constructor.
-  + eapply SynthΠMatch. exact vty'. assumption.
-  + simpl. f_equal; assumption.
-- (* Annotate sum match. *)
-  inv orig. rename v0 into x. rename v1 into y.
-  apply vLemma in H6. destruct H6 as [v' [vty' vsame]]. 
-  apply IHc1 in H7. destruct H7 as [c1' [c1ty' c1same]].
-  apply IHc2 in H8. destruct H8 as [c2' [c2ty' c2same]].
-  exists (CAnnot (ΣMatch v' x c1' y c2') C). constructor.
-  + apply SynthCAnnot. eapply CheckΣMatch. exact vty'. 
-    eapply CheckCBySynth. exact c1ty'. reflexivity.
-    eapply CheckCBySynth. exact c2ty'. reflexivity.
-  + simpl. f_equal; assumption.
-- inv orig.
-  apply vLemma in H2. destruct H2 as [v1' [v1ty' v1same]]. 
-  apply vLemma in H4. destruct H4 as [v2' [v2ty' v2same]].
-  exists (App v1' v2'). constructor.
-  + eapply SynthApp. exact v1ty'. apply CheckVBySynth. assumption.
-  + simpl. f_equal; assumption.
-- inv orig. (* Annotate operations! *)
-  apply vLemma in H6. destruct H6 as [v' [vty' vsame]].
-  apply IHc in H7. destruct H7 as [c' [cty' csame]].
-  exists (CAnnot (Op o v' v0 c') (CTy A Σ eqs)). constructor.
-  + eapply SynthCAnnot. eapply CheckOp. exact H5.
-    apply CheckVBySynth. assumption. eapply CheckCBySynth. exact cty'. auto.
-  + simpl. f_equal; assumption.
-- inv orig. rename v into f. rename v0 into x.
-  apply IHc1 in H6. destruct H6 as [c1' [c1ty' c1same]].
-  apply IHc2 in H7. destruct H7 as [c2' [c2ty' c2same]].
-  exists (LetRec f x (TyFun A C0) c1' c2'). constructor.
-  + apply SynthLetRec. eapply CheckCBySynth. exact c1ty'. auto. assumption.
-  + simpl. f_equal; assumption.
-- inv orig.
-- inv orig.
-  apply vLemma in H2. destruct H2 as [v' [vty' vsame]].
-  apply IHc in H4. destruct H4 as [c' [cty' csame]].
-  exists (Handle v' c'). constructor.
-  + eapply SynthHandle. exact vty'. eapply CheckCBySynth. exact cty'. auto.
-  + simpl. f_equal; assumption.
-- inv orig.
-  apply IHc in H3. destruct H3 as [c' [cty' csame]].
-  exists (CAnnot c' C). constructor.
-  + apply SynthCAnnot. eapply CheckCBySynth. exact cty'. auto.
-  + simpl. auto.
-}{
-clear hLemma.
-revert Γ Σ D. induction h; intros Γ Σ D orig.
-- inv orig. exists CasesØ. constructor. apply CheckCasesØ. reflexivity.
-- inv orig. rename v into x. rename v0 into k.
-  apply IHh in H8. destruct H8 as [h' [hty' hsame]].
-  apply cLemma in H9. destruct H9 as [c' [cty' csame]].
-  exists (CasesU h' o x k c'). constructor.
-  + apply CheckCasesU.
-    * assert (forall h h',
-        h_remove_annot h = h_remove_annot h' ->
-        find_op_case h o = None -> find_op_case h' o = None ).
-      intros H. induction H; intros H' eq nocase; destruct H'.
-      ++ assumption.
-      ++ simpl in eq. discriminate.
-      ++ simpl in eq. discriminate.
-      ++ simpl in eq. injection eq. intros. subst.
-         simpl in *. destruct (o==o1). discriminate.
-         apply IHhcases; assumption.
-      ++ eapply H. exact hsame. assumption.
-    * assumption.
-    * eapply CheckCBySynth. exact cty'. auto.
-  + simpl. f_equal; assumption.
-}
-Qed.
-
