language_formalisation/type_system/erasure.v
@@ -1,0 +1,198 @@
+
+Ltac inv H := inversion H; clear H; subst.
+
+
+Fixpoint vcheck_has_vtype Γ v A {struct v}:
+  vcheck Γ v A -> has_vtype Γ (v_remove_annot v) A
+with vsynth_has_vtype Γ v A {struct v}:
+  vsynth Γ v A -> has_vtype Γ (v_remove_annot v) A
+with ccheck_has_ctype Γ c C {struct c}:
+  ccheck Γ c C -> has_ctype Γ (c_remove_annot c) C
+with csynth_has_ctype Γ c C {struct c}:
+  csynth Γ c C -> has_ctype Γ (c_remove_annot c) C
+with hcheck_has_htype Γ h Σ D {struct h}:
+  hcheck Γ h Σ D -> has_htype Γ (h_remove_annot h) Σ D.
+Proof.
+{
+clear vcheck_has_vtype.
+revert Γ A. induction v; intros Γ A orig; inv orig; try inv H; simpl.
++ apply TypeVar. assumption.
++ apply TypeUnit.
++ apply TypeInt.
++ apply TypeInl. apply IHv. assumption.
++ apply TypeInr. apply IHv. assumption.
++ apply TypePair; auto.
++ apply TypeFun. auto.
++ apply TypeHandler; auto.
++ auto.
+}{
+clear vsynth_has_vtype.
+revert Γ A. induction v; intros Γ A orig; inv orig; simpl.
++ apply TypeVar. assumption.
++ apply TypeUnit.
++ apply TypeInt.
++ apply TypePair; auto.
++ auto.
+}{
+clear ccheck_has_ctype.
+revert Γ C. induction c; intros Γ C orig; inv orig; try inv H; simpl.
++ apply TypeRet. auto.
++ eapply TypeΠMatch. apply vsynth_has_vtype; exact H5.
+  apply csynth_has_ctype. assumption.
++ eapply TypeΣMatch. apply vsynth_has_vtype; exact H6. auto. auto.
++ eapply TypeApp. apply vsynth_has_vtype. exact H3. auto.
++ eapply TypeOp; try exact H5 || auto.
++ eapply TypeLetRec. apply IHc1. exact H7. auto.
++ eapply TypeHandle. apply vsynth_has_vtype. exact H3. auto.
++ auto. 
+}{
+clear csynth_has_ctype.
+revert Γ C. induction c; intros Γ C orig; inv orig; simpl.
++ apply TypeRet. auto.
++ eapply TypeΠMatch. apply vsynth_has_vtype; exact H4. auto.
++ eapply TypeApp. apply vsynth_has_vtype; exact H2. auto.
++ eapply TypeLetRec. apply ccheck_has_ctype. exact H6. auto.
++ eapply TypeHandle. apply vsynth_has_vtype; exact H2. auto.
++ auto.
+}{
+clear hcheck_has_htype.
+revert Γ Σ D. induction h; intros Γ Σ D orig; inv orig; simpl.
++ apply TypeCasesØ.
++ apply TypeCasesU; auto. rewrite <-find_op_remove_annot.
+  rewrite H7. simpl. reflexivity.
+}
+Qed.
+
+
+Fixpoint has_vtype_vsynths_with_annot Γ v A {struct v}:
+  has_vtype Γ v A -> 
+    exists v', vsynth Γ v' A /\ v = v_remove_annot v'
+with has_ctype_csynths_with_annot Γ c C {struct c}:
+  has_ctype Γ c C ->
+    exists c', csynth Γ c' C /\ c = c_remove_annot c'
+with has_htype_hchecks_with_annot Γ h Σ D {struct h}:
+  has_htype Γ h Σ D ->
+    exists h', hcheck Γ h' Σ D /\ h = h_remove_annot h'.
+Proof.
+all:
+rename has_vtype_vsynths_with_annot into vLemma;
+rename has_ctype_csynths_with_annot into cLemma;
+rename has_htype_hchecks_with_annot into hLemma.
+{
+clear vLemma.
+revert Γ A. induction v; intros Γ A orig.
+- destruct v as (name, num).
+  exists (Ann_Var (name, num)). constructor.
+  + apply SynthVar. inv orig. assumption.
+  + reflexivity.
+- exists Ann_Unit. constructor.
+  + inv orig. apply SynthUnit.
+  + reflexivity.
+- exists (Ann_Int t). constructor.
+  + inv orig. apply SynthInt.
+  + reflexivity.
+- (* Annotate sumtypes *)
+  inv orig. apply IHv in H1. destruct H1 as [v' [vty' same]].
+  exists (Ann_Val (Ann_Inl v') (TyΣ A0 B)). constructor.
+  + apply SynthVAnnot. apply CheckInl. apply CheckVBySynth. assumption.
+  + simpl. f_equal. assumption.
+- (* Annotate sumtypes *)
+  inv orig. apply IHv in H1. destruct H1 as [v' [vty' same]].
+  exists (Ann_Val (Ann_Inr v') (TyΣ A0 B)). constructor.
+  + apply SynthVAnnot. apply CheckInr. apply CheckVBySynth. assumption.
+  + simpl. f_equal. assumption.
+- inv orig.
+  apply IHv1 in H2. destruct H2 as [v1' [v1ty' same1]].
+  apply IHv2 in H4. destruct H4 as [v2' [v2ty' same2]].
+  exists (Ann_Pair v1' v2'). constructor.
+  + apply SynthPair; assumption.
+  + simpl. f_equal; assumption.
+- inv orig. (* Annotate functions. *)
+  apply cLemma in H3. destruct H3 as [c' [cty' same]].
+  exists (Ann_Val (Ann_Fun v c') (TyFun A0 C)). constructor.
+  + apply SynthVAnnot. apply CheckFun. eapply CheckCBySynth. exact cty'. auto.
+  + simpl. f_equal. assumption.
+- inv orig. (* Annotate functions. *)
+  apply cLemma in H4. destruct H4 as [c_r' [cty' samec]].
+  apply hLemma in H5. destruct H5 as [h' [hty' sameh]].
+  exists (Ann_Val (Ann_Handler v c_r' h') (TyHandler (CTy A0 sig eqs) D)).
+  constructor.
+  + apply SynthVAnnot. apply CheckHandler;
+    try eapply CheckCBySynth; auto. auto.
+  + simpl. f_equal; assumption.
+}{
+clear cLemma.
+revert Γ C. induction c; intros Γ C orig.
+- inv orig.
+  apply vLemma in H1. destruct H1 as [v' [vty' same]].
+  exists (Ann_Ret v'). constructor.
+  + apply SynthRet. assumption.
+  + simpl. f_equal. assumption.
+- inv orig.
+  apply vLemma in H4. destruct H4 as [v' [vty' same]].
+  apply IHc in H5. destruct H5 as [c' [cty' csame]].
+  exists (Ann_ΠMatch v' (x,y) c'). constructor.
+  + eapply SynthΠMatch. exact vty'. assumption.
+  + simpl. f_equal; assumption.
+- (* Annotate sum match. *)
+  inv orig. rename v0 into x. rename v1 into y.
+  apply vLemma in H6. destruct H6 as [v' [vty' vsame]]. 
+  apply IHc1 in H7. destruct H7 as [c1' [c1ty' c1same]].
+  apply IHc2 in H8. destruct H8 as [c2' [c2ty' c2same]].
+  exists (Ann_Comp (Ann_ΣMatch v' x c1' y c2') C). constructor.
+  + apply SynthCAnnot. eapply CheckΣMatch. exact vty'. 
+    eapply CheckCBySynth. exact c1ty'. reflexivity.
+    eapply CheckCBySynth. exact c2ty'. reflexivity.
+  + simpl. f_equal; assumption.
+- inv orig.
+  apply vLemma in H2. destruct H2 as [v1' [v1ty' v1same]]. 
+  apply vLemma in H4. destruct H4 as [v2' [v2ty' v2same]].
+  exists (Ann_App v1' v2'). constructor.
+  + eapply SynthApp. exact v1ty'. apply CheckVBySynth. assumption.
+  + simpl. f_equal; assumption.
+- inv orig. (* Annotate operations! *)
+  apply vLemma in H6. destruct H6 as [v' [vty' vsame]].
+  apply IHc in H7. destruct H7 as [c' [cty' csame]].
+  exists (Ann_Comp (Ann_Op o v' v0 c') (CTy A Σ eqs)). constructor.
+  + eapply SynthCAnnot. eapply CheckOp. exact H5.
+    apply CheckVBySynth. assumption. eapply CheckCBySynth. exact cty'. auto.
+  + simpl. f_equal; assumption.
+- inv orig. rename v into f. rename v0 into x.
+  apply IHc1 in H5. destruct H5 as [c1' [c1ty' c1same]].
+  apply IHc2 in H6. destruct H6 as [c2' [c2ty' c2same]].
+  exists (Ann_LetRec f x (TyFun A C0) c1' c2'). constructor.
+  + apply SynthLetRec. eapply CheckCBySynth. exact c1ty'. auto. assumption.
+  + simpl. f_equal; assumption.
+- inv orig.
+- inv orig.
+  apply vLemma in H2. destruct H2 as [v' [vty' vsame]].
+  apply IHc in H4. destruct H4 as [c' [cty' csame]].
+  exists (Ann_Handle v' c'). constructor.
+  + eapply SynthHandle. exact vty'. eapply CheckCBySynth. exact cty'. auto.
+  + simpl. f_equal; assumption.
+}{
+clear hLemma.
+revert Γ Σ D. induction h; intros Γ Σ D orig.
+- inv orig. exists Ann_CasesØ. constructor. apply CheckCasesØ. reflexivity.
+- inv orig. rename v into x. rename v0 into k.
+  apply IHh in H8. destruct H8 as [h' [hty' hsame]].
+  apply cLemma in H9. destruct H9 as [c' [cty' csame]].
+  exists (Ann_CasesU h' o x k c'). constructor.
+  + apply CheckCasesU.
+    * assert (forall h h',
+        h = h_remove_annot h' ->
+        find_op_case h o = None -> find_op_ann_case h' o = None ).
+      intros H. induction H; intros H' eq nocase; destruct H'.
+      ++ simpl. reflexivity.
+      ++ simpl in eq. discriminate.
+      ++ simpl in eq. discriminate.
+      ++ simpl in eq. injection eq. intros. subst.
+         simpl in *. destruct (o==o1). discriminate.
+         apply IHhcases. reflexivity. assumption.
+      ++ eapply H. exact hsame. assumption.
+    * assumption.
+    * eapply CheckCBySynth. exact cty'. auto.
+  + simpl. f_equal; assumption.
+}
+Qed.
+
